Working on the max computation.

Isabelle2/AutoRefTest.thy
@@ -92,14 +92,23 @@ section {* The paxos computation *}
   
 definition inst_votes where 
   "inst_votes f i A \<equiv> {(v,b) . \<exists> a \<in> A . \<exists> h . f a = Some h \<and> h i = Some (Some (v,b))}"
+  
+definition inst_inv where 
+  "inst_inv vs vbo \<equiv> case vbo of Some (v,b) \<Rightarrow> (vs \<noteq> {} \<and> (v,b) \<in> vs \<and> b = Max (snd ` vs))
+    | None \<Rightarrow> vs = {}"
+  
+lemma inst_votes_union:
+  "inst_votes f i (A \<union> B) = inst_votes f i A \<union> inst_votes f i B"
+  by (auto simp add:inst_votes_def)
 
 definition inv :: "('a \<rightharpoonup> (nat \<rightharpoonup> (('v \<times> nat) option))) \<Rightarrow> (nat \<rightharpoonup> ('v \<times> nat)) 
-    \<Rightarrow> 'a set \<Rightarrow> nat set \<Rightarrow> bool"  
-  where "inv f g A I \<equiv> \<forall> i \<in> I . \<forall> v b . (g i = Some (v,b)) \<longleftrightarrow>
-    (let vs_i = inst_votes f i A in vs_i \<noteq> {} \<and> (v,b) \<in> vs_i \<and> b = Max (snd ` vs_i))"
+  \<Rightarrow> 'a set \<Rightarrow> nat set \<Rightarrow> bool"  
+  where "inv f g A I \<equiv> (\<forall> i \<in> I . let vs_i = inst_votes f i A in inst_inv vs_i (g i))"
   
 definition spec :: "('a \<rightharpoonup> (nat \<rightharpoonup> (('v \<times> nat) option))) \<Rightarrow> (nat \<rightharpoonup> ('v \<times> nat)) nres" 
   where "spec f \<equiv> SPEC (\<lambda> g . inv f g UNIV UNIV)"
+ (*
+definition inner_loop :: "('a\<times>) 'i \<rightharpoonup> ('v \<times> 'b)" where "inner_loop" *)
   
 definition impl_1 :: "('a \<rightharpoonup> ('i \<rightharpoonup> (('v \<times> 'b::linorder) option))) \<Rightarrow> ('i \<rightharpoonup> ('v \<times> 'b)) nres"
   where "impl_1 f \<equiv>
@@ -110,6 +119,28 @@ definition impl_1 :: "('a \<rightharpoonup> ('i \<rightharpoonup> (('v \<times> 
         | Some (v2,b2) \<Rightarrow> if b \<ge> b2 then r2(i \<mapsto> (v,b)) else r2))) r)
   Map.empty"
   
+lemma step_insert_image_iff:
+  assumes "f ` it \<subseteq> S" and "(k,v) \<in> it" and "\<And> k v1 v2 . \<lbrakk>(k,v1) \<in> it; (k,v2)\<in> it\<rbrakk> \<Longrightarrow> v1 = v2" 
+    and "\<And> k1 k2 v1 v2 . k1 \<noteq> k2 \<Longrightarrow> f (k1,v1) \<noteq> f (k2,v2)"
+  shows "S - f ` (it - {(k,v)}) = insert (f (k,v)) (S - f ` it)"
+proof -
+  have "f ` (it - {(k,v)}) = (f ` it) - f ` {(k,v)}" 
+    using \<open>(k,v) \<in> it\<close> assms(3,4) by auto (blast, metis)
+  thus "S - f ` (it - {(k,v)}) = insert (f (k,v)) (S - (f ` it))"
+    using \<open>f ` it \<subseteq> S\<close> and \<open>(k,v) \<in> it\<close> by (simp add: it_step_insert_iff) 
+qed
+
+lemma it_step_insert_image_fst_iff:
+  assumes  "fst ` it \<subseteq> S" and "(k,v) \<in> it" and "it \<subseteq> map_to_set m"
+  shows "S - fst ` (it - {(k,v)}) = insert (fst (k,v)) (S - fst ` it)"
+proof -
+  have 1:"\<And> k v1 v2 . \<lbrakk>(k,v1) \<in> it; (k,v2)\<in> it\<rbrakk> \<Longrightarrow> v1 = v2" using \<open>it \<subseteq> map_to_set m\<close>
+    by (meson Refine_Misc.map_to_set_inj subsetCE)
+  have 2:"\<And> k1 k2 v1 v2 . k1 \<noteq> k2 \<Longrightarrow> fst (k1,v1) \<noteq> fst (k2,v2)"
+    by simp
+  from step_insert_image_iff[OF assms(1,2) 1 2] show ?thesis by auto
+qed
+
 lemma 
   fixes f::"('a::finite \<rightharpoonup> (nat \<rightharpoonup> (('v \<times> nat) option)))"
   assumes "\<And> a . a \<in> dom f \<Longrightarrow> finite (dom (the (f a)))"
@@ -119,16 +150,101 @@ lemma
   apply (refine_vcg FOREACH_rule[where  
         I="\<lambda> it r . let as = (UNIV::'a set) - (fst ` it) in inv f r as UNIV"])
      apply (simp add:finite_map_to_set)
-    apply (auto simp add:map_to_set_def inv_def Let_def inst_votes_def)[1]
+    apply (auto simp add:map_to_set_def inv_def Let_def inst_votes_def inst_inv_def)[1]
    defer apply simp
-  subgoal premises prems for kv it s a fa using prems
-  apply (refine_vcg FOREACH_rule[where 
-        I="\<lambda> it2 r2 . let is = (dom s - dom fa) \<union> (dom fa) - (fst ` it2); 
-          as = UNIV - fst ` (it - {kv}) in inv f r2 as is"])
-       apply (simp add:finite_map_to_set; fastforce simp add:map_to_set_def)
-    (* First problem is that we need to show that the max remains unchanged for
-      instances not in dom fa *)
-    oops
+  subgoal premises prems for kv it s a fa
+  proof -
+    define as' where "as' \<equiv> UNIV - fst ` (it - {kv})"
+    define as where "as \<equiv> UNIV - fst ` it"
+    have 1:"as' = (insert a as)" unfolding as_def as'_def
+      using it_step_insert_image_fst_iff[of it UNIV a fa] \<open>kv \<in> it\<close> \<open>it \<subseteq> map_to_set f\<close>
+      by (auto simp add:\<open>kv = (a, fa)\<close>)
+    have 2:"f a = Some fa" using  \<open>kv = (a,fa)\<close> \<open>it \<subseteq> map_to_set f\<close> \<open>kv \<in> it\<close> by auto
+        (metis (mono_tags, lifting) in_pair_collect_simp map_to_set_def mem_Collect_eq subset_Collect_conv)
+    have 3:"inv f s as UNIV" using as_def prems(4) by auto
+    have 4:"fa2 = fa" if "(a,fa2) \<in> it" for fa2 using \<open>kv = (a,fa)\<close> \<open>it \<subseteq> map_to_set f\<close> \<open>kv \<in> it\<close> that
+        by (metis (no_types, lifting) Refine_Misc.map_to_set_inj subsetCE)
+    define inner where "inner \<equiv> 
+      FOREACH (map_to_set fa) (\<lambda> (i,vbo) r2 . RETURN 
+        (case vbo of None \<Rightarrow> r2 | Some (v,b) \<Rightarrow>
+          (case r2 i of None \<Rightarrow> r2(i \<mapsto> (v,b))
+          | Some (v2,b2) \<Rightarrow> if b \<ge> b2 then r2(i \<mapsto> (v,b)) else r2))) s"
+    have "inner \<le> SPEC (\<lambda>r. inv f r as' UNIV)" unfolding inner_def
+      apply (refine_vcg FOREACH_rule[where I="\<lambda> it2 r2 . let 
+            is_1 = (dom s \<inter> (fst ` it2)) \<union> (dom s - dom fa); is_2 = ((dom s \<union> dom fa) - (fst ` it2)) in
+            inv f r2 as' is_2 \<and> inv f r2 as is_1 \<and> (fst ` it2) \<subseteq> dom fa"])
+      subgoal using "2" assms finite_map_to_set by fastforce
+      subgoal unfolding Let_def (* The invariant is true of the initial state *)
+      proof (intro conjI)
+        let ?is_1="(dom s \<inter> fst ` map_to_set fa) \<union> (dom s - dom fa)"
+        let ?is_2="(dom s \<union> dom fa) - fst ` map_to_set fa"
+        have "?is_2 = dom s - dom fa" by (simp add: Un_Diff map_to_set_dom) 
+        show "inv f s as' ?is_2" unfolding inv_def Let_def
+        proof 
+          fix i
+          assume "i \<in> ?is_2"
+          hence "fa i = None"  by (auto simp add:\<open>?is_2 = dom s - dom fa\<close>)
+          hence "inst_votes f i {a} = {}" using \<open>f a = Some fa\<close> by (simp add:inst_votes_def)
+          hence "inst_votes f i as' = inst_votes f i as" by (auto simp add: \<open>as' = insert a as\<close> inst_votes_def)
+          thus "inst_inv (inst_votes f i as') (s i)" using \<open>inv f s as UNIV\<close> by (simp add:inv_def)
+        qed  
+        show "inv f s as ?is_1" using \<open>inv f s as UNIV\<close> by (simp add:inv_def)
+        show "fst ` map_to_set fa \<subseteq> dom fa" by (simp add: map_to_set_dom)
+      qed
+      subgoal premises prems for kv2 it2 s2 i hi (* The inductive step. *)
+        unfolding Let_def
+      proof (intro conjI)
+        thm prems
+        define s3 where "s3 \<equiv> (case hi of None \<Rightarrow> s2 | Some (v, b) \<Rightarrow>
+          (case s2 i of None \<Rightarrow> s2(i \<mapsto> (v, b))
+          | Some (v2, b2) \<Rightarrow> if b2 \<le> b then s2(i \<mapsto> (v, b)) else s2))"
+        define is_2' where "is_2' \<equiv> (dom s \<union> dom fa) - (fst ` (it2 - {kv2}))"
+        define is_2 where "is_2 \<equiv> (dom s \<union> dom fa) - (fst ` it2)"
+        define is_1 where "is_1 \<equiv> (dom s \<inter> fst ` it2) \<union> (dom s - dom fa)"
+        define is_1' where "is_1' \<equiv> (dom s \<inter> fst ` (it2 - {kv2})) \<union> (dom s - dom fa)"
+        have 5:"is_2' = insert i is_2"  
+        proof -
+          have "fst ` it2 \<subseteq> (dom s \<union> dom fa)" using \<open>it2 \<subseteq> map_to_set fa\<close> by (auto simp add: map_to_set_dom)
+          with it_step_insert_image_fst_iff[of it2 "dom s \<union> dom fa" i hi] \<open>it2 \<subseteq> map_to_set fa\<close> \<open>kv2 = (i,hi)\<close> \<open>kv2 \<in> it2\<close> 
+          show ?thesis by (auto simp add:is_2'_def is_2_def)
+        qed
+        have 6:"inv f s2 as' is_2" unfolding is_2_def using prems(3) by auto
+        have 7:"inv f s2 as is_1" unfolding is_1_def by (meson prems(3))
+        have 8:"fa i = Some hi" using \<open>kv2 = (i,hi)\<close> \<open>it2 \<subseteq> map_to_set fa\<close> \<open>kv2 \<in> it2\<close>
+          by (metis (mono_tags, lifting) in_pair_collect_simp map_to_set_def mem_Collect_eq subset_Collect_conv)
+        have 9:"hi2 = hi" if "(i,hi2) \<in> it2" for hi2 using \<open>kv2 = (i,hi)\<close> \<open>it2 \<subseteq> map_to_set fa\<close> \<open>kv2 \<in> it2\<close> that
+          by (metis (no_types, lifting) Refine_Misc.map_to_set_inj subsetCE)
+        have 10:"i \<notin> is_2" using \<open>kv2 \<in> it2\<close> \<open>kv2 = (i,hi)\<close> unfolding is_2_def by (simp add: img_fst)
+        have 11:"is_1' \<subseteq> is_1 - {i}" unfolding is_1_def is_1'_def using "5" is_2'_def "8" by blast
+        have 12:"fst ` it2 \<subseteq> dom fa" by (meson prems(3))
+        have "AutoRefTest.inv f s3 as' is_2'"
+        proof (auto simp add:inv_def)
+          fix j
+          assume "j \<in> is_2'"
+          define vs' where "vs' \<equiv> inst_votes f j as'"
+          define vs where "vs \<equiv> inst_votes f j as"
+          have 4:"vs' = (inst_votes f j {a}) \<union> vs" unfolding vs'_def vs_def by (metis "1" insert_is_Un inst_votes_union) 
+          show "inst_inv vs' (s3 j)"
+          proof (cases "i = j")
+            case True
+            show ?thesis
+            proof (cases hi)
+              case None
+              hence "inst_votes f j {a} = {}" unfolding inst_votes_def using "8" 2 \<open>i=j\<close> by auto
+              hence "vs' = vs" using "4" by blast 
+              moreover have "s3 j = s2 j" by (simp add: None s3_def)
+              moreover have "inst_inv vs (s2 j)"
+              proof -
+                have "j \<in> is_1 \<or> j \<in> (fst ` it2) - dom s"
+              ultimately show ?thesis by auto
+            next
+              case (Some a)
+              then show ?thesis sorry
+            qed
+          next
+            case False
+            show ?thesis
+        oops
   
   
 schematic_goal impl_1:
